change the main method to my original way

nmap_assign.thy
@@ -1,11 +1,8 @@
-theory nmap_assign
+theory nmap_assign   
 imports
   nmap_expr
 begin
 
-(***
-typedef '\<alpha> proc  = "UNIV :: (bool, '\<alpha> \<times> '\<alpha>) uexpr set" ..
-***)
 type_synonym '\<alpha> proc        = " (bool, '\<alpha> \<times> '\<alpha>) uexpr"
 type_synonym ('\<alpha>, '\<beta>) urel  = " (bool, '\<alpha> \<times> '\<beta>) uexpr"
 
@@ -19,9 +16,16 @@ adhoc_overloading
 
 consts uskip :: "'a" ("II")
 definition skip_r :: " '\<alpha> proc " where "skip_r = assigns_r id"
+print_theorems
 adhoc_overloading
   uskip skip_r
-    
+
+
+
+
+
+
+
 syntax
   \<comment> \<open> Single and multiple assignement \<close>
   "_assignment"     :: "svids \<Rightarrow> uexprs \<Rightarrow> '\<alpha> proc"  ("'(_') := '(_')")  
@@ -37,16 +41,27 @@ translations
   "_assignment x v" <= "_assignment (_spvar x) v"
   "x,y := u,v" <= "CONST uassigns (CONST subst_upd (CONST subst_upd (CONST id) (CONST svar x) u) (CONST svar y) v)"
 
+lemma " \<langle>[y \<mapsto>\<^sub>s f]\<rangle>\<^sub>a =  y := f "
+  by (simp add: pr_var_def)
+
+
+
+
 (***    test begin    ***)
 lemma assign_skip:
   assumes "vwb_lens x"
   shows "(x := &x) = II"
-  by (metis assms pr_var_def skip_r_def usubst_upd_pr_var_id)
+proof -
+  have " [x \<mapsto>\<^sub>s var x] = id"
+    by (simp add: assms usubst_upd_var_id)
+  then show ?thesis
+    by (simp add: assms skip_r_def usubst_upd_var_id)
+qed
 
 lemma assigns_simul2:
   assumes "vwb_lens x"
   shows "(x,x) := (u,v) = (x := v)"
-  by (simp add: assms usubst_upd_idem)
+  by (simp add: assms  usubst_upd_idem)
 
 lemma assign_simul1:
   assumes "vwb_lens y" "x \<bowtie> y"
@@ -54,6 +69,25 @@ lemma assign_simul1:
   by (metis assms(1) assms(2) one_add_one pr_var_def usubst_upd_comm usubst_upd_pr_var_id)
 
 
+
+
+
+
+
+
+
+
+
+(**
+
+consts useq     :: "'a \<Rightarrow> 'b \<Rightarrow> 'c" (infixr ";;" 61)
+lift_definition seqr::"('\<alpha>, '\<beta>) urel \<Rightarrow> ('\<beta>, '\<gamma>) urel \<Rightarrow>  (bool,'\<alpha> \<times> '\<gamma>) uexpr"
+is "\<lambda> P Q b. b \<in> ({p. P p} O {q. Q q})" .
+adhoc_overloading
+  useq seqr
+
+
+lemma assigns_comp: "(assigns_r f ;; assigns_r g) = assigns_r (g \<circ> f)" 
 
 
 
@@ -74,7 +108,7 @@ class nchoice =
   assumes nch_assoc   : "(x \<sqinter> y) \<sqinter> z = x \<sqinter> (y \<sqinter> z)"
       and nch_commute : "x \<sqinter> y = y \<sqinter> x"
       and nch_idemp   : "(x \<sqinter> x) = x" 
-(**
+
       and nch_skip_left: " II \<sqinter> x = x"
       and nch_skip_right: "x \<sqinter>  II = x"
 **)
@@ -92,7 +126,7 @@ lemma (in nchoice) "(x:=3)  \<sqinter> (y:=4) =  (y:=4)  \<sqinter>  (x:=3)"
 
 lemma " (a:=3)  \<sqinter> (b:=4) =  (b:=4)  \<sqinter>  (a:=3)  "
 'a  = 'b state_scheme
-***)
+
 
 
 
@@ -103,7 +137,7 @@ definition ifprog :: " 'a  \<Rightarrow> bool \<Rightarrow> 'a  \<Rightarrow> 'a
 
 theorem ifprog_idemp : "x \<triangleleft> boole \<triangleright>\<^sub>\<p> x = x"
   by (simp add: ifprog_def)
-
+***)
 
 
 
