nmap_test.thy
@@ -20,6 +20,15 @@ theorem "(a,b) := (2+3, &b) = (a,b) := (5,&b)"
 theorem "(a,b,c) := (2, &b, 4) = (a,c) := (2,4)"
   by (metis b_vwb_lens pr_var_def state_indeps(1) usubst_upd_comm usubst_upd_var_id)
 
+theorem  "(a := 4 ;; a := &a + 2) = (a := 6)"
+  by (simp add: hellerqweqweo_test)
+
+lemma assigns_cobbmp: "a := 3;; (b := 3 ;; c := 3) = (a := 3 ;; b := 3) ;; c := 3" 
+  by (simp add: assigns_cobbmp)
+
+
+
+
 theorem "(a:=5) \<triangleleft> True \<triangleright>\<^sub>\<p> (b:=6) = (a:=5)"
   by (simp add: ifprog_def)
 
